Progress on Hacl.Impl.ECIES

code/experimental/ecies/Hacl.Impl.ECIES.fst
@@ -14,15 +14,18 @@ module Seq = Lib.Sequence
 module Loops = Lib.LoopCombinators
 module Spec = Spec.ECIES
 
-(* module SHA2 = Hacl.Impl.SHA2_256 *)
-(* module HMAC = Hacl.Impl.HMAC_SHA2_256 *)
-(* module HKDF = Hacl.Impl.HKDF_SHA2_256 *)
 
-
-assume val crypto_random: output:buffer uint8 -> len:size_t ->
+val crypto_random: output:buffer uint8 -> len:size_t{v len > 0 /\ length output == v len} ->
   Stack bool
   (requires (fun h -> live h output))
   (ensures  (fun h0 _ h1 -> modifies1 output h0 h1))
+
+let crypto_random output len =
+  push_frame ();
+  let tmp = create len (u8 0xAB) in
+  copy output tmp;
+  pop_frame ();
+  true
 
 
 
@@ -38,19 +41,32 @@ let id_of_ciphersuite = u8 0
 ///
 
 inline_for_extraction
+let size_id_of_ciphersuite = size 1
+
+inline_for_extraction
 let size_nonce = size (Spec.ECIES.size_nonce ciphersuite)
+
+inline_for_extraction
+let size_aead_key = size 32
+
+inline_for_extraction
+let size_aead_nonce = size 16
 
 inline_for_extraction
 let size_key = size (Spec.ECIES.size_key ciphersuite)
 
 inline_for_extraction
+let size_key_dh = size (Spec.ECIES.size_key_dh ciphersuite)
+
+inline_for_extraction
+let size_ecies_secret = 1ul +. size_key +. 2ul *. size_key_dh
+
+inline_for_extraction
 let size_context = size 32
 
 inline_for_extraction
-let size_info = size 32
+let size_info = size_id_of_ciphersuite + (size Spec.ECIES.size_label_key) + size_context
 
-inline_for_extraction
-let size_key_dh = size (Spec.ECIES.size_key_dh ciphersuite)
 
 
 ///
@@ -74,35 +90,40 @@ let const_label_key: x:ilbuffer size_t (size Spec.ECIES.size_label_key){witnesse
 
 
 val encap:
-    output: lbuffer uint8 (1ul +. size_key +. 2ul *. size_key_dh)
-  -> kpub: key_public_p
+    output: lbuffer uint8 size_ecies_secret
+  -> pk: key_public_p
   -> context: lbuffer uint8 size_context ->
   Stack unit
-  (requires (fun h -> live h output /\ live h kpub /\ live h context
-                 /\ disjoint output kpub /\ disjoint output context))
+  (requires (fun h -> live h output /\ live h pk /\ live h context
+                 /\ disjoint output pk /\ disjoint output context))
   (ensures  (fun h0 _ h1 -> modifies1 output h0 h1))
 
-let encap output kpub context =
+let encap output pk context =
   push_frame ();
   let flag = sub output (size 0) (size 1) in
   let key = sub output (size 1) size_key in
-  let eph_kpub = sub output (1ul +. size_key) size_key_dh in
-  let eph_kpriv = sub output (1ul +. size_key +. size_key_dh) size_key_dh in
+  let epk = sub output (1ul +. size_key) size_key_dh in
+  let esk = create size_key_dh (u8 0) in
   let extracted = create size_key (u8 0) in
   let secret = create size_key (u8 0) in
   let salt = create (2ul *. size_key_dh) (u8 0) in
   let info = create size_info (u8 0) in
-  let res0 = crypto_random eph_kpriv size_key_dh in
-  Hacl.Curve25519_64.ecdh res1 eph_kpub eph_kpriv;
-  Hacl.Curve25519_64.ecdh res2 secret eph_kpriv kpub;
-  update_sub salt (size 0) size_key_dh eph_kpub;
-  update_sub salt size_key_dh size_key_dh kpub;
+  let res0 = crypto_random esk size_key_dh in
+  (* let epk = DH.secret_to_public (curve_of_cs cs) esk in *)
+  Hacl.Curve25519_64.secret_to_public epk esk;
+  Hacl.Curve25519_64.ecdh secret esk pk;
+  (* let salt = epk @| pk in *)
+  update_sub salt (size 0) size_key_dh epk;
+  update_sub salt size_key_dh size_key_dh pk;
+  (* let extracted = HKDF.hkdf_extract (hash_of_cs cs) salt secret in *)
   Hacl.HKDF_SHA2_256.hkdf_extract extracted salt (2ul *. size_key_dh) secret size_key;
+  (* let info = (id_of_cs cs) @| label_key @| context in *)
   info.(0ul) <- id_of_ciphersuite;
-  update_sub info (size 1) Spec.ECIES.size_label_key const_label_key;
-  update_sub info Spec.ECIES.size_label_key size_context context;
+  update_sub info (size 1) (size Spec.ECIES.size_label_key) const_label_key;
+  update_sub #MUT #uint8 #size_info info (1ul +. Spec.ECIES.size_label_key) size_context context;
+  (* let key = HKDF.hkdf_expand (hash_of_cs cs) extracted info (size_key cs) in *)
   Hacl.HKDF_SHA2_256.hkdf_expand key extracted size_key info size_info size_key;
-  if res0 && res1 && res2 then output.(0ul) <- (u8 0) else output.(0ul) <- (u8 1);
+  if res0 then output.(0ul) <- (u8 0) else output.(0ul) <- (u8 1);
   pop_frame ()
 
 
@@ -110,69 +131,60 @@ val decap:
     output: lbuffer uint8 (size_key +. 1ul)
   -> kpriv: key_private_p
   -> eph_kpub: key_public_p
-  -> context: lbuffer uint8 size_context
+  -> context: lbuffer uint8 size_context ->
   Stack unit
   (requires (fun h -> live h output /\ live h kpriv /\ live h eph_kpub /\ live h context))
   (ensures  (fun h0 _ h1 -> modifies1 output h0 h1))
 
-let decap output kpriv eph_kpub context =
+let decap output sk epk context =
   push_frame();
-  let kpub = create size_key_public (u8 0) in
-  let salt = create (2ul *. size_key_public) (u8 0) in
+  let pk = create size_key_dh (u8 0) in
+  let salt = create (2ul *. size_key_dh) (u8 0) in
   let info = create size_info (u8 0) in
   let extracted = create size_key (u8 0) in
   let flag = sub output (size 0) (size 1) in
-  let secret = sub output (size 1) size_secret in
-  let res1 = secret_to_public kpub kpriv in
-  let res2 = DH.dh secret kpriv eph_kpub in
-  update_sub salt (size 0) size_key_public eph_kpub;
-  update_sub salt size_key_public size_key_public kpub;
-  HKDF.extract extracted salt (2ul *. size_key_public) secret size_secret;
+  let secret = sub output (size 1) size_ecies_secret in
+  (* let pk = DH.secret_to_public (curve_of_cs cs) sk in *)
+  Hacl.Curve25519_64.secret_to_public pk sk;
+  Hacl.Curve25519_64.ecdh secret sk epk;
+  (* let salt = epk @| pk in *)
+  update_sub salt (size 0) size_key_dh epk;
+  update_sub salt size_key_dh size_key_dh pk;
+  (* let extracted = HKDF.hkdf_extract (hash_of_cs cs) salt secret in *)
+  Hacl.HKDF_SHA2_256.hkdf_extract extracted salt (2ul *. size_key_dh) secret size_ecies_secret;
+  (* let info = (id_of_cs cs) @| label_key @| context in *)
   info.(0ul) <- id_of_ciphersuite;
-  update_sub info (size 1) size_label_key const_label_key;
-  update_sub info size_label_key size_context context;
-  HKDF.expand secret extracted size_secret info size_info size_key;
+  update_sub info (size 1) (size Spec.ECIES.size_label_key) const_label_key;
+  update_sub #MUT #uint8 #size_info info (1ul +. size Spec.ECIES.size_label_key) size_context context;
+  (* let key = HKDF.hkdf_expand (hash_of_cs cs) extracted info (size_key cs) in *)
+  Hacl.HKDF_SHA2_256.hkdf_expand secret extracted size_key info size_info size_key;
   pop_frame()
-
-
-
-val encrypt:
-    cs: ciphersuite
-  -> sk: key_s cs
-  -> input: bytes{length input <= max_size_t
-           /\ length input + AEAD.size_block (aead_of_cs cs) <= max_size_t
-           /\ length input + AEAD.padlen (aead_of_cs cs) (length input) <= max_size_t}
-  -> aad: bytes {length aad <= max_size_t /\ length aad + AEAD.padlen (aead_of_cs cs) (length aad) <= max_size_t}
-  -> counter: uint32 ->
-  Tot bytes
-
-let encrypt cs sk input aad counter =
-  let klen = AEAD.size_key (aead_of_cs cs) in
-  let key = sub sk 0 klen in
-  let nonce = sub sk klen (size_nonce cs - numbytes U32) in
-  let ctr = uint_to_bytes_le counter in
-  AEAD.aead_encrypt (aead_of_cs cs) key (nonce @| ctr) input aad
 
 
 val encrypt:
     output: buffer uint8
-  -> sk: key_secret_s
+  -> sk: lbuffer uint8 size_key_dh
   -> input: buffer uint8
-  -> len: size_t{v len == length input
-               /\ length input <= max_size_t
-               /\ length input + AEAD.size_block (aead_of_cs cs) <= max_size_t
-               /\ length input + AEAD.padlen (aead_of_cs cs) (length input) <= max_size_t}
+  -> len: size_t{v len == length input}
   -> aad: buffer uint8
-  -> alen: size_t{v alen == length aad
-               /\ length aad <= max_size_t
-               /\ length aad + AEAD.padlen (aead_of_cs cs) (length aad) <= max_size_t}
+  -> alen: size_t{v alen == length aad}
   -> counter: uint32 ->
   Stack unit
   (requires (fun h -> live h output /\ live h sk /\ live h input /\ live h aad
                  /\ disjoint output sk /\ disjoint output input /\ disjoint output aad))
   (ensures  (fun h0 _ h1 -> modifies1 output h0 h1))
 
-let encrypt output sk input len aad alen counter = admit()
-  (* push_frame(); *)
-  (* let ctr8 = create (numbytes U32) (u8 0) in *)
+let encrypt output sk input len aad alen counter =
+  push_frame();
+  let ctr8 = create (numbytes U32) (u8 0) in
+  let aead_nonce = create size_aead_nonce (u8 0) in
   (* let key = sub sk (size 0) size_ *)
+  let key = sub sk 0ul size_aead_key in
+  (* let nonce = sub sk klen (size_nonce cs - numbytes U32) in *)
+  let nonce = sub sk size_aead_key (size_aead_nonce - numbytes U32) in
+  let ctr = uint_to_bytes_le ctr8 counter in
+  (* let aead_nonce = (nonce @| ctr) in *)
+  update_sub aead_nonce 0ul (size_aead_nonce - numbytes U32) nonce;
+  update_sub aead_nonce (size_aead_nonce - numbytes U32) (numbytes U32) ctr8;
+  Hacl.AesGCM.NI.encrypt input aad
+  (* AEAD.aead_encrypt (aead_of_cs cs) key (nonce @| ctr) input aad *)
